share/steel/examples/pulse/parallel/NewDomains.fsti
@@ -9,6 +9,7 @@ open Pulse.Lib.Core
 module HR = Pulse.Lib.HigherReference
 open FStar.List.Tot.Base
 open GhostTaskQueue
+open Promises
 
 type comp_task (t: task_elem) =
   unit -> stt t._1 (own_None t._2) (fun _ -> own_None t._2)
@@ -18,7 +19,7 @@ let task_queue: Type u#1 = list (t:task_elem & comp_task t)
 let inv_task_queue
   (q: HR.ref task_queue) // the task queue
   (c: ref int) // a counter of how many tasks are currently being performed
-  (r: ghost_mono_ref task_elem)
+  (r: erased (ghost_mono_ref task_elem))
   : vprop
 = (exists_ (fun vq ->
   exists_ (fun vc -> 
@@ -26,13 +27,15 @@ let inv_task_queue
     //** cond_deadline r (map dfst vq) vc // TODO: Remove
     )))
 
-let par_env = (q: HR.ref task_queue & c: ref int & r: ghost_mono_ref task_elem & Lock.lock (inv_task_queue q c r))
+let par_env = (q: HR.ref task_queue & c: ref int & r: erased (ghost_mono_ref task_elem) & Lock.lock (inv_task_queue q c r))
 
-val get_mono_list (p: par_env): ghost_mono_ref task_elem
+val get_mono_list (p: par_env): erased (ghost_mono_ref task_elem)
 
 let pure_handler a (p: par_env)
   = (res: ref (option a) & Lock.lock (own_res res)
   & t: erased task_elem & pos:erased nat & erased (certificate (get_mono_list p) t pos))
+
+let deadline_env (p: par_env) = deadline (get_mono_list p)
 
 val spawn_emp
   (#a:Type0)
@@ -40,12 +43,15 @@ val spawn_emp
   (ct: current_task (p._3)) // should be erased
   (f: (par_env -> ct:erased (current_task p._3) -> unit -> stt a (is_active ct) (fun _ -> is_active ct)))
   // TODO: remove par_env arg
-: stt (pure_handler a p) (is_active ct) (fun _ -> is_active ct)
+: stt (pure_handler a p) (is_active ct)
+  (fun h -> is_active ct ** 
+promise (deadline_env p) (exists_ (fun f -> (exists_ (fun v ->
+    pts_to (reveal h._3)._2 #f v ** pure (Some? v))))))
 
 val join_emp (#a:Type0) (p: par_env) (h: pure_handler a p)
 : stt a emp (fun _ -> emp)
 
-val worker (p: par_env): stt unit emp (fun () -> deadline (get_mono_list p))
+val worker (p: par_env): stt unit emp (fun () -> deadline_env p)
 
 (*
 fn par_block_pulse_emp' (#a: Type0)
