share/steel/examples/pulse/parallel/GhostTaskQueuePoolAlive.fsti
@@ -1,0 +1,118 @@
+module GhostTaskQueuePoolAlive
+
+module L = FStar.List.Tot.Base
+module P = FStar.Preorder
+module GR = Pulse.Lib.GhostReference
+
+type task_status = | Todo | Ongoing | Done
+type task_with_status (a: Type) = a & task_status
+type mono_list (a: Type) = list (task_with_status a)
+//val mono_list (a: Type): Type
+
+(*
+let small_inv (r: ghost_mono_ref task_elem) (q: list task_elem) (c: int): vprop 
+= exists_ (fun l -> pts_to_ghost_queue_half r l **
+  tasks_res_own l one_half **
+  pure (count_ongoing l = c /\ get_actual_queue l == q)
+  ** (if c = 0 && L.length q = 0 then deadline r
+  else pts_to_ghost_queue_half r l ** tasks_res_own l one_quart)
+)
+*)
+
+open Pulse.Lib.Pervasives
+
+module Lock = Pulse.Lib.SpinLock
+
+let one_quart = half_perm (half_perm full_perm)
+
+let own_res (#a: Type0) (r: ref (option a)) = (exists_ (fun v -> pts_to r #one_quart v))
+
+let three_quart = sum_perm (half_perm full_perm) (half_perm (half_perm full_perm))
+
+let own_None r = pts_to r #three_quart None
+
+let task_elem: Type u#1 = (
+  a: Type0 // return type of the computation
+  & r: ref (option a) // the reference where we put the result of the computation
+  & Lock.lock (own_res r)//(exists_ (fun v -> pts_to r half v ** (if None? v then pts_to r half v else emp)))
+)
+
+
+//val ghost_mono_ref (a: Type u#1): Type0
+//let gmref = erased (ghost_mono_ref task_elem)
+
+val pool: Type // implemented as a ghost mono ref and a ghost bool ref
+
+val certificate (p:pool) (t: task_elem) (pos: nat): Type0
+let secret_certificate (p: pool) (t: task_elem): Type0 = (pos: nat & certificate p t pos)
+
+val deadline (p: pool): vprop // ghost bool ref, false
+
+val duplicate_deadline (p: pool):
+stt_ghost unit emp_inames (deadline p) (fun () -> deadline p ** deadline p)
+
+val small_inv (p: pool) (q: list task_elem) (c: int): vprop 
+
+val pool_alive (f: perm) (p: pool): vprop // f/2 permission to the ghost bool ref, true
+
+// 0. init queue with task
+val init_ghost_queue: stt_ghost pool emp_inames emp (fun p -> small_inv p [] 0)
+
+// 1. enqueue task
+val spawn_task_ghost
+(p: pool)
+(q: list task_elem) (c: int)
+(t: task_elem)
+(#f: perm)
+: stt_ghost (secret_certificate p t) emp_inames
+(small_inv p q c ** pts_to t._2 #three_quart None ** pool_alive f p)
+(fun _ -> small_inv p (t::q) c ** pool_alive f p)
+
+// 2. pop task todo
+val pop_task_ghost
+(p: pool)
+(t: task_elem)
+(q: list task_elem) (c: int)
+: stt_ghost (secret_certificate p t) emp_inames
+(small_inv p (t::q) c)
+(fun _ -> small_inv p q (c + 1) ** pts_to t._2 #three_quart None)
+
+(*
+val prove_task_ongoing
+  (#t: task_elem)
+  (#pos: nat)
+  (#v: option t._1)
+  (r:gmref)
+  (q: list task_elem) (c: int)
+  (w:certificate r t pos)
+: stt_ghost unit emp_inames
+(small_inv r q c ** pts_to t._2 #three_quart v)
+(fun () -> small_inv r q c ** pts_to t._2 #three_quart v ** pure (c > 0))
+
+val prove_ongoing_non_neg
+  (r: gmref)
+  (q: list task_elem) (c: int)
+: stt_ghost unit emp_inames
+(small_inv r q c)
+(fun () -> small_inv r q c ** pure (c >= 0))
+*)
+
+// 3. conclude a task
+val conclude_task_ghost
+(#t: task_elem)
+(#pos: nat)
+(p: pool)
+(q: list task_elem) (c: int)
+(x: t._1)
+(w: secret_certificate p t):
+stt_ghost unit emp_inames
+(small_inv p q c ** pts_to t._2 #three_quart (Some x))
+(fun () -> small_inv p q (c - 1)) //imp_vprop (c = 1 && L.length q = 0) (deadline r))
+
+val proof_promise (#t: task_elem) (#pos: nat)
+  (p: pool)
+  (w:secret_certificate p t)
+: stt_ghost unit emp_inames
+(deadline p)
+(fun () -> deadline p ** (exists_ (fun f -> (exists_ (fun v ->
+                          pts_to t._2 #f v ** pure (Some? v))))))
